src/interfaces/rationals.v
@@ -1,10 +1,15 @@
 Require Import
-  abstract_algebra interfaces.integers natpair_integers.
+  abstract_algebra interfaces.integers natpair_integers
+  theory.fields.
 
-Class Rationals A {e plus mult opp zero one mult_inv } `{∀ x y: A, Decision (x = y)} {inj_inv}: Prop :=
-  { rationals_field:> @Field A e plus mult opp zero one mult_inv
+Section rationals.
+  Context A `{field : Field A} `{∀ x y: A, Decision (x = y)}.
+
+  Class Rationals {inj_inv}: Prop :=
+  { rationals_field:> Field A
   ; rationals_frac: Surjective (λ p, integers_to_ring (Z nat) A (fst p) * / integers_to_ring (Z nat) A (snd p)) (inv:=inj_inv)
   ; rationals_embed_ints: Injective (integers_to_ring (Z nat) A) }.
+End rationals.
 
 (* rational_embed_ints is not declared as a coercion because we prove a stronger result in a moment *)
 
